src/examples/matmul-tile/Kuiper.MatMulTile.Prep.fst
@@ -1,7 +1,7 @@
 module Kuiper.MatMulTile.Prep
+#set-options "--fuel 1 --ifuel 1 --z3rlimit 40"
 #lang-pulse
 
-#set-options "--fuel 1 --ifuel 1 --z3rlimit 40"
 
 open Kuiper
 open Kuiper.Math
@@ -24,33 +24,34 @@ fn setup
   (rows shared columns : pos)
   (bdim : pos { bdim /? rows /\ bdim /? columns /\ bdim /? shared /\ bdim < pow2 30})
   (nblk : nat { nblk == (rows / bdim) * (columns / bdim) })
-  (nthr : nat { nthr == bdim * bdim
-                     /\ nblk * nthr == rows * columns
-                     /\ 2 * (shared / bdim) >= 0
-                     })
+  (nthr : nat { nthr == bdim * bdim })
   (* ^ 2nd and 3rd conjunct above just to help verifying this spec, sigh. *)
-  (ga1 : gpu_array u64 (rows * shared))
-  (ga2 : gpu_array u64 (shared * columns))
-  (gr  : gpu_array u64 (nblk * nthr))
-  (v1 : seq u64 { len v1 == rows * shared })
-  (v2 : seq u64 { len v2 == shared * columns })
-  (#s : seq u64)
-  requires gpu_pts_to_array gr s **
-           gpu_pts_to_array ga1 v1 **
-           gpu_pts_to_array ga2 v2
-  ensures  bigstar 0 (nblk * nthr) (fun i ->
-             K.kpre rows shared columns ga1 ga2 gr #v1 #v2 (nblk * nthr)
-               (K.tid_to_idx rows shared columns bdim i))
+  (ga : gpu_array u64 (rows * shared))
+  (gb : gpu_array u64 (shared * columns))
+  (gr : gpu_array u64 (rows * columns))
+  requires
+    (ga |-> 'va) **
+    (gb |-> 'vb) **
+    (gr |-> 'vr)
+  ensures 
+    bigstar 0 (nblk * nthr) (fun i ->
+      Kernel.kpre rows shared columns ga gb gr #'va #'vb (nblk * nthr)
+        (Kernel.tid_to_idx rows shared columns bdim i))
 {
+  assert (pure (nblk * nthr == rows * columns)); // silly
+  gpu_pts_to_ref ga;
+  gpu_pts_to_ref gb;
+  gpu_pts_to_ref gr;
   // Sharing the input matrices (splitting permissions)
-  fold I.gpu_pts_to_matrix rows   shared  ga1 1 v1;
-  fold I.gpu_pts_to_matrix shared columns ga2 1 v2;
-  I.gpu_matrix_share_underspec #_ #1 rows   shared  ga1 (nblk * nthr) v1;
-  I.gpu_matrix_share_underspec #_ #2 shared columns ga2 (nblk * nthr) v2;
+  fold I.gpu_pts_to_matrix rows   shared  ga 1 'va;
+  fold I.gpu_pts_to_matrix shared columns gb 1 'vb;
+  I.gpu_matrix_share_underspec #_ #1 rows   shared  ga (nblk * nthr) 'va;
+  I.gpu_matrix_share_underspec #_ #2 shared columns gb (nblk * nthr) 'vb;
 
   // Sharing the output matrix (splitting each cell)
-  gpu_pts_to_ref gr; (* obtain length v == (nblk * nthr) *)
-  gpu_array_slice_1 #4 gr;
+  // NB: We set the implicit to get a bigstar for 0 to nblk*nthr, isntead
+  // of rows*columns. This seems to work better given the pains of NLarith.
+  gpu_array_slice_1 #4 #_ #(nblk * nthr) gr;
 
   // Join resources into a single bigstar
   bigstar_zip #1 #2 #3 0 (nblk * nthr) _ _;
@@ -60,11 +61,11 @@ fn setup
   ghost
   fn aux (i:nat{0 <= i /\ i < (nblk * nthr)})
     requires
-      I.gpu_pts_to_matrix rows   shared  ga1 (nblk * nthr) v1 **
-      I.gpu_pts_to_matrix shared columns ga2 (nblk * nthr) v2 **
-      gpu_pts_to_array_slice gr i (i + 1) seq![s `Seq.index` i]
+      I.gpu_pts_to_matrix rows   shared  ga (nblk * nthr) 'va **
+      I.gpu_pts_to_matrix shared columns gb (nblk * nthr) 'vb **
+      gpu_pts_to_array_slice gr i (i + 1) seq!['vr `Seq.index` i]
     ensures
-      K.kpre rows shared columns ga1 ga2 gr #v1 #v2 (nblk * nthr) i
+      K.kpre rows shared columns ga gb gr #'va #'vb (nblk * nthr) i
   {
     fold gpu_pts_to_array1 gr i;
     ()
@@ -75,15 +76,15 @@ fn setup
     rows * columns;
   };
   bigstar_map #_ #_ #0 #(nblk * nthr) aux;
-  lemma_nonneg_mul (nblk) (nthr);
+  lemma_nonneg_mul nblk nthr;
   lemma_divides_exact rows bdim;
   lemma_divides_exact columns bdim;
   assert (pure (rows / bdim >= 1));
   assert (pure (columns / bdim >= 1));
   bigstar_permute #0 #0 #(nblk * nthr) #_ (K.permute (rows/bdim) (columns/bdim) bdim);
   ghost fn rewrite_permute_to_fn (i: nat {0 <= i /\ i < (nblk * nthr)})
-    requires K.kpre rows shared columns ga1 ga2 gr #v1 #v2 (nblk * nthr) ((K.permute (rows/bdim) (columns/bdim) bdim).f i)
-    ensures  K.kpre rows shared columns ga1 ga2 gr #v1 #v2 (nblk * nthr) (K.tid_to_idx rows shared columns bdim i)
+    requires K.kpre rows shared columns ga gb gr #'va #'vb (nblk * nthr) ((K.permute (rows/bdim) (columns/bdim) bdim).f i)
+    ensures  K.kpre rows shared columns ga gb gr #'va #'vb (nblk * nthr) (K.tid_to_idx rows shared columns bdim i)
   {
     ()
   };
@@ -101,19 +102,19 @@ fn breakdown
                      /\ 2 * (shared / bdim) >= 0
                      })
   (* ^ 2nd and 3rd conjunct above just to help verifying this spec, sigh. *)
-  (ga1 : gpu_array u64 (rows * shared))
-  (ga2 : gpu_array u64 (shared * columns))
-  (gr  : gpu_array u64 (nblk * nthr))
-  (v1 : seq u64 { len v1 == rows * shared })
-  (v2 : seq u64 { len v2 == shared * columns })
+  (ga : gpu_array u64 (rows * shared))
+  (gb : gpu_array u64 (shared * columns))
+  (gr : gpu_array u64 (rows * columns))
   requires
     bigstar 0 (nblk * nthr) (fun i ->
-      K.kpost rows shared columns ga1 ga2 gr #v1 #v2 (nblk * nthr) (K.tid_to_idx rows shared columns bdim i))
+      K.kpost rows shared columns ga gb gr #'va #'vb (nblk * nthr) (K.tid_to_idx rows shared columns bdim i))
   ensures
-    (exists* vr. gpu_pts_to_array gr vr) **
-    gpu_pts_to_array ga1 v1 **
-    gpu_pts_to_array ga2 v2
+    (exists* vr. gr |-> vr) **
+    (ga |-> 'va) **
+    (gb |-> 'vb)
 {
+  assert (pure (nblk * nthr == rows * columns)); // silly
+
   lemma_nonneg_mul nblk nthr;
   lemma_divides_exact rows bdim;
   lemma_divides_exact columns bdim;
@@ -127,8 +128,8 @@ fn breakdown
   let perm = perm_inv (K.permute (rows/bdim) (columns/bdim) bdim);
   bigstar_permute #0 #0 #(nblk * nthr) #_ perm;
   ghost fn rewrite_permute_to_fn (i: nat {0 <= i /\ i < (nblk * nthr)})
-    requires K.kpost rows shared columns ga1 ga2 gr #v1 #v2 (nblk * nthr) (perm.f (K.tid_to_idx rows shared columns bdim i))
-    ensures  K.kpost rows shared columns ga1 ga2 gr #v1 #v2 (nblk * nthr) i
+    requires K.kpost rows shared columns ga gb gr #'va #'vb (nblk * nthr) (perm.f (K.tid_to_idx rows shared columns bdim i))
+    ensures  K.kpost rows shared columns ga gb gr #'va #'vb (nblk * nthr) i
   {
     let once: (j: nat{ 0 <= j /\ j < (nblk * nthr) }) = K.tid_to_idx rows shared columns bdim i;
     let once': (j: nat{ 0 <= j /\ j < (nblk * nthr) }) = perm.g i;
@@ -151,10 +152,10 @@ fn breakdown
   gpu_array_unslice_1_underspec #4 gr #1.0R;
 
   // Unsharing the input matrices (gathering permissions)
-  I.gpu_matrix_unshare_underspec #_ #1 rows   shared  ga1 (nblk * nthr) v1;
-  I.gpu_matrix_unshare_underspec #_ #2 shared columns ga2 (nblk * nthr) v2;
-  unfold I.gpu_pts_to_matrix rows   shared  ga1 1 v1;
-  unfold I.gpu_pts_to_matrix shared columns ga2 1 v2;
+  I.gpu_matrix_unshare_underspec #_ #1 rows   shared  ga (nblk * nthr) 'va;
+  I.gpu_matrix_unshare_underspec #_ #2 shared columns gb (nblk * nthr) 'vb;
+  unfold I.gpu_pts_to_matrix rows   shared  ga 1 'va;
+  unfold I.gpu_pts_to_matrix shared columns gb 1 'vb;
 
   ()
 }
