src/examples/matmul-tile/Kuiper.MatMulTile.Prep.fsti
@@ -1,37 +1,31 @@
 module Kuiper.MatMulTile.Prep
-#lang-pulse
-
 #set-options "--fuel 1 --ifuel 1 --z3rlimit 40"
+#lang-pulse
 
 open Kuiper
 open Kuiper.Math
 
-module SZ   = FStar.SizeT
-module Kernel = Kuiper.MatMulTile.Kernel
+module SZ = FStar.SizeT
+module K  = Kuiper.MatMulTile.Kernel
 
 ghost
 fn setup
   (rows shared columns : pos)
   (bdim : pos { bdim /? rows /\ bdim /? columns /\ bdim /? shared /\ bdim < pow2 30})
   (nblk : nat { nblk == (rows / bdim) * (columns / bdim) })
-  (nthr : nat { nthr == bdim * bdim
-                     /\ nblk * nthr == rows * columns
-                     /\ 2 * (shared / bdim) >= 0
-                     })
+  (nthr : nat { nthr == bdim * bdim })
   (* ^ 2nd and 3rd conjunct above just to help verifying this spec, sigh. *)
-  (ga1 : gpu_array u64 (rows * shared))
-  (ga2 : gpu_array u64 (shared * columns))
-  (gr  : gpu_array u64 (nblk * nthr))
-  (v1 : seq u64 { len v1 == rows * shared })
-  (v2 : seq u64 { len v2 == shared * columns })
-  (#s : seq u64)
-  requires gpu_pts_to_array gr s **
-           gpu_pts_to_array ga1 v1 **
-           gpu_pts_to_array ga2 v2
-  ensures  bigstar 0 (nblk * nthr) (fun i ->
-             Kernel.kpre rows shared columns ga1 ga2 gr #v1 #v2 (nblk * nthr)
-               (Kernel.tid_to_idx rows shared columns bdim i))
-
+  (ga : gpu_array u64 (rows * shared))
+  (gb : gpu_array u64 (shared * columns))
+  (gr : gpu_array u64 (rows * columns))
+  requires
+    (ga |-> 'va) **
+    (gb |-> 'vb) **
+    (gr |-> 'vr)
+  ensures 
+    bigstar 0 (nblk * nthr) (fun i ->
+      K.kpre rows shared columns ga gb gr #'va #'vb (nblk * nthr)
+        (K.tid_to_idx rows shared columns bdim i))
 
 ghost
 fn breakdown
@@ -43,15 +37,13 @@ fn breakdown
                      /\ 2 * (shared / bdim) >= 0
                      })
   (* ^ 2nd and 3rd conjunct above just to help verifying this spec, sigh. *)
-  (ga1 : gpu_array u64 (rows * shared))
-  (ga2 : gpu_array u64 (shared * columns))
-  (gr  : gpu_array u64 (nblk * nthr))
-  (v1 : seq u64 { len v1 == rows * shared })
-  (v2 : seq u64 { len v2 == shared * columns })
+  (ga : gpu_array u64 (rows * shared))
+  (gb : gpu_array u64 (shared * columns))
+  (gr : gpu_array u64 (rows * columns))
   requires
     bigstar 0 (nblk * nthr) (fun i ->
-      Kernel.kpost rows shared columns ga1 ga2 gr #v1 #v2 (nblk * nthr) (Kernel.tid_to_idx rows shared columns bdim i))
+      K.kpost rows shared columns ga gb gr #'va #'vb (nblk * nthr) (K.tid_to_idx rows shared columns bdim i))
   ensures
-    (exists* vr. gpu_pts_to_array gr vr) **
-    gpu_pts_to_array ga1 v1 **
-    gpu_pts_to_array ga2 v2
+    (exists* vr. gr |-> vr) **
+    (ga |-> 'va) **
+    (gb |-> 'vb)
